theories/L/Complexity/Cook/FSAT_to_SAT.v
@@ -1,0 +1,41 @@
+From PslBase Require Import Base. 
+From Undecidability.L.Complexity.Cook Require Import Prelim FSAT SAT.
+(*From Undecidability.L.Complexity Require Import Tactics. *)
+From Undecidability.L.Datatypes Require Import LLists. 
+Require Import Lia. 
+
+(*v <-> (v1 ∧ v2) *)
+Definition tseytinAnd (v v1 v2 : var) : cnf := 
+[[(false, v); (true, v1)]; [(false, v); (true, v2)]; [(false, v1); (false, v2); (true, v)]].
+(*v <-> (v1 ∨ v2)*)
+Definition tseytinOr (v v1 v2 : var) : cnf := 
+  [[(false, v); (true, v1); (true, v2)]; [(false, v1); (true, v)]; [(false, v2); (true, v)]].
+(* v <-> ¬ v'*)
+Definition tseytinNot (v v' : var) : cnf := 
+  [[(false, v); (false, v')]; [(true, v); (true, v')]].
+
+Fixpoint tseytin' (nfVar : var) (f : formula) : (var * cnf * var) := 
+  match f with 
+  | Ftrue => (nfVar, [[nfVar]], S nfVar)
+  | Fvar v => (v, [[]], nfVar)
+  | For f1 f2 => let
+      '(rv1, N1, nfVar1) := tseytin' nfVar f1 in let 
+      '(rv2, N2, nfVar2) := tseytin' nfVar1 f2 in 
+      (nfVar2, N1 ++ N2 ++ tseytinOr nfVar2 rv1 rv2, S nfVar2)
+  | Fand f1 f2 => let
+      '(rv1, N1, nfVar1) := tseytin' nfVar f1 in let
+      '(rv2, N2, nfVar2) := tseytin' nfVar1 f2 in 
+      (nfVar2, N1 ++ N2 ++ tseytinAnd nfVar2 rv1 rv2, S nfVar2)
+  | Fneg f => let
+      '(rv, N, nfVar') := tseytin' nfVar f in 
+      (nfVar', N ++ tseytinNot nfVar' rv, S nfVar')
+  end. 
+
+Definition tseytin f : var * cnf := 
+  let '(repVar, N, _) := tseytin' (S (formula_maxVar f)) f in (repVar, N). 
+
+(*a variable v represents a formula f with respect to a CNF N iff the CNF with the variable v assumed to be true is equisatisfiable to f*)
+Definition formula_repr (f : formula) (N : cnf) (v : var) := FSAT f <-> SAT ([(true, v)] :: N). 
+
+Definition 
+
